src/test.lean
@@ -1,0 +1,137 @@
+import alc
+
+namespace test
+
+open ALC
+open ALC.Concept
+
+
+inductive ac : Type
+ | man : ac
+ | woman : ac
+
+inductive ar : Type
+ | hasChild : ar
+
+@[reducible]
+def ic : ac → set ℕ  
+ | ac.man   := ({2,4} : set ℕ)
+ | ac.woman := ({1,3} : set ℕ)     
+
+@[reducible]
+def ir : ar → set (ℕ × ℕ)
+ | ar.hasChild := ({(1,2),(4,3)} : set (ℕ × ℕ))
+
+@[reducible]
+def i := Interpretation.mk ℕ ic ir
+
+-- below, the concept is not reduced to {2,4} but to a equivalent λ-term.
+
+#reduce interp i (Concept.Atomic ac.woman)
+
+#reduce interp i (Some (Role.Atomic ar.hasChild) (Concept.Atomic ac.man))
+
+
+-- instead of 'compute' concepts, let us proof things about the interpretation
+
+example : 
+ interp i (Some (Role.Atomic ar.hasChild) (Concept.Atomic ac.man)) = ({1} : set ℕ) :=
+begin
+ dsimp [interp,r_interp,i],
+ rw [ic,ir],
+ ext n,  
+ apply iff.intro,
+ { intro h1, 
+   simp at *, 
+   apply (exists.elim h1),
+   simp, intros a ha hb,
+   finish,
+ },
+ { intros h1,
+   norm_num at h1,
+   rw h1,
+   apply exists.intro 2,
+   finish,
+ } 
+end
+
+-- Mario's proof
+example :
+  interp i (Every (Role.Atomic ar.hasChild) (Concept.Atomic ac.man)) = ({4}ᶜ : set ℕ) :=
+begin
+  ext n,
+  simp [interp, r_interp, ir, ic],
+  split,
+  { rintro h rfl,
+    have := h 3, revert this,
+    norm_num, 
+  },
+  { rintro h _ (⟨rfl, rfl⟩|⟨rfl, rfl⟩), {norm_num},
+    cases h rfl },
+end
+
+-- if i, ic and ir were not 'reducible'
+example :
+  interp i (Every (Role.Atomic ar.hasChild) (Concept.Atomic ac.man)) = ({4}ᶜ : set ℕ) :=
+begin
+  dsimp [i, interp],
+  ext n,
+  simp [r_interp, ir],
+  split,
+  { rintro H rfl,
+    have := H 3, revert this,
+    norm_num },
+  { rintro h _ (⟨rfl, rfl⟩|⟨rfl, rfl⟩), {norm_num},
+    cases h rfl },
+end
+
+-- a detailed proof
+example :
+  interp i (Every (Role.Atomic ar.hasChild) (Concept.Atomic ac.man)) = ({4}ᶜ : set ℕ) :=
+begin
+  ext n,
+  simp [interp, r_interp, ir, ic],
+  split,
+  { rintro h rfl,
+    have := h 3, revert this,
+    norm_num, 
+  },
+  { intros h1 a h2,
+    cases h2 with h2a h2b,
+    exact or.inl h2a.2,
+    exfalso, exact h1 h2b.left,
+  },
+end
+
+
+
+-- detailed proofs for the steps closed with 'finish' above.
+
+example (h : 1 = 4) : false := 
+begin
+ -- if succ 0 = succ 3 then 0 = 3 because succ is injective
+ have h1 := (nat.succ_injective h),
+ apply nat.succ_ne_zero _ h1.symm, 
+end
+
+
+example (n a : ℕ) (ha : n = 1 ∧ a = 2 ∨ n = 4 ∧ a = 3)
+  (hb : a = 2 ∨ a = 4) : n = 1 := 
+begin
+ by_contradiction,
+ cases hb with hb1 hb2,
+ cases ha with ha1 ha2,
+ exact h ha1.1, 
+ have hx := and.intro ha2.2 hb1,
+ finish,
+ finish,
+end
+
+
+example (α : Type*) (p q : α → Prop) : (∀ x : α, p x ∧ q x) → ∀ y : α, p y  :=
+begin
+ intros h x,
+ exact (h x).1,
+end
+
+end test
